Revert "Update gh-pages branch with current main (#632)"
This reverts commit efe92b2687b1548b74ba7e5fb8fbd045a24ff2fe.

silveroak-opentitan/aes/Acorn/AESSV.hs
@@ -32,4 +32,5 @@ main = do writeSystemVerilog aes_mix_columns_Netlist
           writeTestBench aes_sub_bytes_tb
           writeSystemVerilog aes_add_round_key_Netlist
           writeTestBench aes_add_round_key_tb
+          writeSystemVerilog cipher_round_Netlist
           writeSystemVerilog aes_cipher_core_Netlist
