tests/AccumulatingAdderEnable/AccumulatingAdderEnable.v
@@ -79,14 +79,14 @@ Local Notation "'#' l" := (map (fun i => N2Bv_sized 8 (N.of_nat i)) l)
 Local Open Scope list_scope.
 
 Example accumulatingAdderEnable_ex1:
-  simulate accumulatingAdderEnable
+  multistep accumulatingAdderEnable
             (combine
                (# [1;1;1;1;1;1;1;1])
                (map nat2bool [1;1;1;1;0;0;0;0])) = # [1;2;3;4;5;5;5;5].
 Proof. reflexivity. Qed.
 
 Example accumulatingAdderEnable_ex2:
-  simulate accumulatingAdderEnable
+  multistep accumulatingAdderEnable
             (combine
                (# [0;1;2;3;4;5;6;7])
                (map nat2bool [0;0;0;1;1;1;0;1])) = # [0;1;2;3;7;12;18;19].
